

# Seminar 4

**THEOREM 12—The Ratio Test** Let  $\sum a_n$  be a series with positive terms and suppose that

$$\lim_{n \rightarrow \infty} \frac{a_{n+1}}{a_n} = \rho.$$

Then **(a)** the series *converges* if  $\rho < 1$ , **(b)** the series *diverges* if  $\rho > 1$  or  $\rho$  is infinite, **(c)** the test is *inconclusive* if  $\rho = 1$ .

**EXAMPLE 1** Investigate the convergence of the following series.

**(b)**  $\sum_{n=1}^{\infty} \frac{(2n)!}{n!n!}$

**(b)** If  $a_n = \frac{(2n)!}{n!n!}$ , then  $a_{n+1} = \frac{(2n+2)!}{(n+1)!(n+1)!}$  and

$$\begin{aligned} \frac{a_{n+1}}{a_n} &= \frac{n!n!(2n+2)(2n+1)(2n)!}{(n+1)!(n+1)!(2n)!} \\ &= \frac{(2n+2)(2n+1)}{(n+1)(n+1)} = \frac{4n+2}{n+1} \rightarrow 4. \end{aligned}$$

The series diverges because  $\rho = 4$  is greater than 1.

**EXAMPLE 1** Investigate the convergence of the following series.

**(a)**  $\sum_{n=0}^{\infty} \frac{2^n + 5}{3^n}$

**Solution** We apply the Ratio Test to each series.

**(a)** For the series  $\sum_{n=0}^{\infty} (2^n + 5)/3^n$ ,

$$\frac{a_{n+1}}{a_n} = \frac{(2^{n+1} + 5)/3^{n+1}}{(2^n + 5)/3^n} = \frac{1}{3} \cdot \frac{2^{n+1} + 5}{2^n + 5} = \frac{1}{3} \cdot \left( \frac{2 + 5 \cdot 2^{-n}}{1 + 5 \cdot 2^{-n}} \right) \rightarrow \frac{1}{3} \cdot \frac{2}{1} = \frac{2}{3}.$$

The series converges because  $\rho = 2/3$  is less than 1. This does *not* mean that  $2/3$  is the sum of the series. In fact,

$$\sum_{n=0}^{\infty} \frac{2^n + 5}{3^n} = \sum_{n=0}^{\infty} \left( \frac{2}{3} \right)^n + \sum_{n=0}^{\infty} \frac{5}{3^n} = \frac{1}{1 - (2/3)} + \frac{5}{1 - (1/3)} = \frac{21}{2}.$$

**THEOREM 13—The Root Test** Let  $\sum a_n$  be a series with  $a_n \geq 0$  for  $n \geq N$ , and suppose that

$$\lim_{n \rightarrow \infty} \sqrt[n]{a_n} = \rho.$$

Then **(a)** the series *converges* if  $\rho < 1$ , **(b)** the series *diverges* if  $\rho > 1$  or  $\rho$  is infinite, **(c)** the test is *inconclusive* if  $\rho = 1$ .

**THEOREM 14—The Alternating Series Test (Leibniz's Test)** The series

$$\sum_{n=1}^{\infty} (-1)^{n+1} u_n = u_1 - u_2 + u_3 - u_4 + \cdots$$

converges if all three of the following conditions are satisfied:

1. The  $u_n$ 's are all positive.
2. The positive  $u_n$ 's are (eventually) nonincreasing:  $u_n \geq u_{n+1}$  for all  $n \geq N$ , for some integer  $N$ .
3.  $u_n \rightarrow 0$ .

**DEFINITION** A series  $\sum a_n$  **converges absolutely** (is **absolutely convergent**) if the corresponding series of absolute values,  $\sum |a_n|$ , converges.

The geometric series in Example 3 converges absolutely because the corresponding series of absolute values

$$\sum_{n=0}^{\infty} \frac{1}{2^n} = 1 + \frac{1}{2} + \frac{1}{4} + \frac{1}{8} + \cdots$$

converges. The alternating harmonic series does not converge absolutely because the corresponding series of absolute values is the (divergent) harmonic series.



## Using the Ratio Test

In Exercises 1–8, use the Ratio Test to determine if each series converges or diverges.

1.  $\sum_{n=1}^{\infty} \frac{2^n}{n!}$

2.  $\sum_{n=1}^{\infty} \frac{n+2}{3^n}$

3.  $\sum_{n=1}^{\infty} \frac{(n-1)!}{(n+1)^2}$

4.  $\sum_{n=1}^{\infty} \frac{2^{n+1}}{n3^{n-1}}$

---

## Using the Root Test

In Exercises 9–16, use the Root Test to determine if each series converges or diverges.

9.  $\sum_{n=1}^{\infty} \frac{7}{(2n+5)^n}$

10.  $\sum_{n=1}^{\infty} \frac{4^n}{(3n)^n}$

11.  $\sum_{n=1}^{\infty} \left( \frac{4n+3}{3n-5} \right)^n$

12.  $\sum_{n=1}^{\infty} \left( \ln \left( e^2 + \frac{1}{n} \right) \right)^{n+1}$

13.  $\sum_{n=1}^{\infty} \frac{8}{(3 + (1/n))^{2n}}$

14.  $\sum_{n=1}^{\infty} \sin^n \left( \frac{1}{\sqrt{n}} \right)$

## Determining Convergence or Divergence

In Exercises 17–44, use any method to determine if the series converges or diverges. Give reasons for your answer.

17.  $\sum_{n=1}^{\infty} \frac{n^{\sqrt{2}}}{2^n}$

18.  $\sum_{n=1}^{\infty} n^2 e^{-n}$

19.  $\sum_{n=1}^{\infty} n! e^{-n}$

20.  $\sum_{n=1}^{\infty} \frac{n!}{10^n}$

21.  $\sum_{n=1}^{\infty} \frac{n^{10}}{10^n}$

22.  $\sum_{n=1}^{\infty} \left( \frac{n-2}{n} \right)^n$

## Determining Convergence or Divergence

In Exercises 1–14, determine if the alternating series converges or diverges. Some of the series do not satisfy the conditions of the Alternating Series Test.

1.  $\sum_{n=1}^{\infty} (-1)^{n+1} \frac{1}{\sqrt{n}}$

2.  $\sum_{n=1}^{\infty} (-1)^{n+1} \frac{1}{n^{3/2}}$

3.  $\sum_{n=1}^{\infty} (-1)^{n+1} \frac{1}{n3^n}$

4.  $\sum_{n=2}^{\infty} (-1)^n \frac{4}{(\ln n)^2}$

5.  $\sum_{n=1}^{\infty} (-1)^n \frac{n}{n^2 + 1}$

6.  $\sum_{n=1}^{\infty} (-1)^{n+1} \frac{n^2 + 5}{n^2 + 4}$



# Seminar 5

**DEFINITIONS**     A **power series about  $x = 0$**  is a series of the form

$$\sum_{n=0}^{\infty} c_n x^n = c_0 + c_1 x + c_2 x^2 + \cdots + c_n x^n + \cdots \tag{1}$$

A **power series about  $x = a$**  is a series of the form

$$\sum_{n=0}^{\infty} c_n (x - a)^n = c_0 + c_1 (x - a) + c_2 (x - a)^2 + \cdots + c_n (x - a)^n + \cdots \tag{2}$$

in which the **center**  $a$  and the **coefficients**  $c_0, c_1, c_2, \dots, c_n, \dots$  are constants.

**THEOREM 18—The Convergence Theorem for Power Series**     If the power series

$\sum_{n=0}^{\infty} a_n x^n = a_0 + a_1 x + a_2 x^2 + \cdots$  converges at  $x = c \neq 0$ , then it converges absolutely for all  $x$  with  $|x| < |c|$ . If the series diverges at  $x = d$ , then it diverges for all  $x$  with  $|x| > |d|$ .

**COROLLARY TO THEOREM 18**     The convergence of the series  $\sum c_n (x - a)^n$  is described by one of the following three cases:

1. There is a positive number  $R$  such that the series diverges for  $x$  with  $|x - a| > R$  but converges absolutely for  $x$  with  $|x - a| < R$ . The series may or may not converge at either of the endpoints  $x = a - R$  and  $x = a + R$ .
2. The series converges absolutely for every  $x$  ( $R = \infty$ ).
3. The series converges at  $x = a$  and diverges elsewhere ( $R = 0$ ).



### How to Test a Power Series for Convergence

1. Use the Ratio Test (or Root Test) to find the interval where the series converges absolutely. Ordinarily, this is an open interval

$$|x - a| < R \quad \text{or} \quad a - R < x < a + R.$$

2. If the interval of absolute convergence is finite, test for convergence or divergence at each endpoint, as in Examples 3a and b. Use a Comparison Test, the Integral Test, or the Alternating Series Test.
3. If the interval of absolute convergence is  $a - R < x < a + R$ , the series diverges for  $|x - a| > R$  (it does not even converge conditionally) because the  $n$ th term does not approach zero for those values of  $x$ .

$R$  is called the **radius of convergence** of the power series, and the interval of radius  $R$  centered at  $x = a$  is called the **interval of convergence**. The interval of convergence may be open, closed, or half-open, depending on the particular series. At points  $x$  with  $|x - a| < R$ , the series converges absolutely. If the series converges for all values of  $x$ , we say its radius of convergence is infinite. If it converges only at  $x = a$ , we say its radius of convergence is zero.

## Operations on Power Series

**THEOREM 19—The Series Multiplication Theorem for Power Series** If  $A(x) = \sum_{n=0}^{\infty} a_n x^n$  and  $B(x) = \sum_{n=0}^{\infty} b_n x^n$  converge absolutely for  $|x| < R$ , and

$$c_n = a_0 b_n + a_1 b_{n-1} + a_2 b_{n-2} + \cdots + a_{n-1} b_1 + a_n b_0 = \sum_{k=0}^n a_k b_{n-k},$$

then  $\sum_{n=0}^{\infty} c_n x^n$  converges absolutely to  $A(x)B(x)$  for  $|x| < R$ :

$$\left( \sum_{n=0}^{\infty} a_n x^n \right) \cdot \left( \sum_{n=0}^{\infty} b_n x^n \right) = \sum_{n=0}^{\infty} c_n x^n.$$

Finding the general coefficient  $c_n$  in the product of two power series can be very tedious and the term may be unwieldy. The following computation provides an illustration of a product where we find the first few terms by multiplying the terms of the second series by each term of the first series:

$$\begin{aligned} & \left( \sum_{n=0}^{\infty} x^n \right) \cdot \left( \sum_{n=0}^{\infty} (-1)^n \frac{x^{n+1}}{n+1} \right) \\ &= (1 + x + x^2 + \cdots) \left( x - \frac{x^2}{2} + \frac{x^3}{3} - \cdots \right) \quad \text{Multiply second series . . .} \\ &= \underbrace{\left( x - \frac{x^2}{2} + \frac{x^3}{3} - \cdots \right)}_{\text{by 1}} + \underbrace{\left( x^2 - \frac{x^3}{2} + \frac{x^4}{3} - \cdots \right)}_{\text{by } x} + \underbrace{\left( x^3 - \frac{x^4}{2} + \frac{x^5}{3} - \cdots \right)}_{\text{by } x^2} + \cdots \\ &= x + \frac{x^2}{2} + \frac{5x^3}{6} - \frac{x^4}{6} \cdots \quad \text{and gather the first four powers.} \end{aligned}$$

We can also substitute a function  $f(x)$  for  $x$  in a convergent power series.



**THEOREM 21—The Term-by-Term Differentiation Theorem** If  $\sum c_n(x - a)^n$  has radius of convergence  $R > 0$ , it defines a function

$$f(x) = \sum_{n=0}^{\infty} c_n(x - a)^n \quad \text{on the interval} \quad a - R < x < a + R.$$

This function  $f$  has derivatives of all orders inside the interval, and we obtain the derivatives by differentiating the original series term by term:

$$f'(x) = \sum_{n=1}^{\infty} n c_n(x - a)^{n-1},$$

$$f''(x) = \sum_{n=2}^{\infty} n(n - 1) c_n(x - a)^{n-2},$$

and so on. Each of these derived series converges at every point of the interval  $a - R < x < a + R$ .

**EXAMPLE 4** Find series for  $f'(x)$  and  $f''(x)$  if

$$f(x) = \frac{1}{1 - x} = 1 + x + x^2 + x^3 + x^4 + \cdots + x^n + \cdots$$

$$= \sum_{n=0}^{\infty} x^n, \quad -1 < x < 1$$

**Solution** We differentiate the power series on the right term by term:

$$f'(x) = \frac{1}{(1 - x)^2} = 1 + 2x + 3x^2 + 4x^3 + \cdots + nx^{n-1} + \cdots$$

$$= \sum_{n=1}^{\infty} nx^{n-1}, \quad -1 < x < 1;$$

$$f''(x) = \frac{2}{(1 - x)^3} = 2 + 6x + 12x^2 + \cdots + n(n - 1)x^{n-2} + \cdots$$

$$= \sum_{n=2}^{\infty} n(n - 1)x^{n-2}, \quad -1 < x < 1$$

**THEOREM 22—The Term-by-Term Integration Theorem**

Suppose that

$$f(x) = \sum_{n=0}^{\infty} c_n (x - a)^n$$

converges for  $a - R < x < a + R$  ( $R > 0$ ). Then

$$\sum_{n=0}^{\infty} c_n \frac{(x - a)^{n+1}}{n + 1}$$

converges for  $a - R < x < a + R$  and

$$\int f(x) dx = \sum_{n=0}^{\infty} c_n \frac{(x - a)^{n+1}}{n + 1} + C$$

for  $a - R < x < a + R$ .**Intervals of Convergence**

In Exercises 1–36, **(a)** find the series' radius and interval of convergence. For what values of  $x$  does the series converge **(b)** absolutely, **(c)** conditionally?

1.  $\sum_{n=0}^{\infty} x^n$

2.  $\sum_{n=0}^{\infty} (x + 5)^n$

3.  $\sum_{n=0}^{\infty} (-1)^n (4x + 1)^n$

4.  $\sum_{n=1}^{\infty} \frac{(3x - 2)^n}{n}$

5.  $\sum_{n=0}^{\infty} \frac{(x - 2)^n}{10^n}$

6.  $\sum_{n=0}^{\infty} (2x)^n$